New benchmark fixes to parse: insert assume true in loop bodies whenever * was used; encode booleans as ints; encode ifs before and after loops as assumes; fix one case where we had quite in variable names

ice-benchmarks/single/fig3.desugared.dimo.bpl
@@ -1,1 +1,38 @@
-(x == y ==> lock == 1)
+implementation main()
+{
+  var x: int;
+  var y: int;
+  var lock: int;
+  var choice: int;
+
+
+  anon0:
+    lock := 0;
+    lock := 1;
+    assume choice == 0 ==> lock == 0 && y == x + 1;
+    assume choice != 0 ==> lock == 1 && y == x;
+    goto anon4_LoopHead;
+
+  anon4_LoopHead:
+    goto anon4_LoopDone, anon4_LoopBody;
+
+  anon4_LoopBody:
+    assume {:partition} x != y;
+    lock := 1;
+    x := y;
+    goto anon5_Then, anon5_Else;
+
+  anon5_Else:
+    goto anon4_LoopHead;
+
+  anon5_Then:
+    lock := 0;
+    y := y + 1;
+    goto anon4_LoopHead;
+
+  anon4_LoopDone:
+    assume {:partition} x == y;
+    assert lock == 1;
+    return;
+}
+
