ice-benchmarks/single/formula22.desugared.dimo.bpl
@@ -1,1 +1,68 @@
-(x1 <= x2 && (x2 >= 0 || x2 - x3 <= 2))
+implementation main()
+{
+  var x1: int;
+  var x2: int;
+  var x3: int;
+  var x4: int;
+  var x5: int;
+  var x6: int;
+  var x7: int;
+  var x8: int;
+  var x1_: int;
+  var x2_: int;
+  var x3_: int;
+  var x4_: int;
+  var x5_: int;
+  var x6_: int;
+  var x7_: int;
+  var x8_: int;
+
+
+  anon0:
+    x1 := 0;
+    x2 := 0;
+    x3 := 0;
+    x4 := 0;
+    x5 := 0;
+    x6 := 0;
+    x7 := 0;
+    x8 := 0;
+    goto anon4_LoopHead;
+
+  anon4_LoopHead:
+    goto anon4_LoopDone, anon4_LoopBody;
+
+  anon4_LoopBody:
+    assume true;
+    havoc x1_;
+    havoc x2_;
+    havoc x3_;
+    havoc x4_;
+    havoc x5_;
+    havoc x6_;
+    havoc x7_;
+    havoc x8_;
+    goto anon5_Then, anon5_Else;
+
+  anon5_Else:
+    assume {:partition} !(x1_ <= x2_ && (x2_ >= 0 || x2_ - x3_ <= 2));
+    goto anon4_LoopHead;
+
+  anon5_Then:
+    assume {:partition} x1_ <= x2_ && (x2_ >= 0 || x2_ - x3_ <= 2);
+    x1 := x1_;
+    x2 := x2_;
+    x3 := x3_;
+    x4 := x4_;
+    x5 := x5_;
+    x6 := x6_;
+    x7 := x7_;
+    x8 := x8_;
+    goto anon4_LoopHead;
+
+  anon4_LoopDone:
+    assume true;
+    assert x1 <= x2 && (x2 >= 0 || x2 - x3 <= 2);
+    return;
+}
+
