ice-benchmarks/single/formula25.dimo.bpl
@@ -4,7 +4,7 @@ procedure main()
 {
 
   var x1, x2, x3, x4, x5, x6, x7, x8: int;
-  var x1', x2', x3', x4', x5', x6', x7', x8': int;
+  var x1_, x2_, x3_, x4_, x5_, x6_, x7_, x8_: int;
 
   x1 := 0;
   x2 := 0;
@@ -18,25 +18,25 @@ procedure main()
   while(*)
   // invariant (x1 <= 0 && x1 >= x4 + 1 && x2 == x3 && (x4 >= 0 || x4 <= x3));
   {
-    havoc x1';
-    havoc x2';
-    havoc x3';
-    havoc x4';
-    havoc x5';
-    havoc x6';
-    havoc x7';
-    havoc x8';
+    havoc x1_;
+    havoc x2_;
+    havoc x3_;
+    havoc x4_;
+    havoc x5_;
+    havoc x6_;
+    havoc x7_;
+    havoc x8_;
 
-    if(x1' <= 0 && x1' >= x4' + 1 && x2' == x3' && (x4' >= 0 || x4' <= x3'))
+    if(x1_ <= 0 && x1_ >= x4_ + 1 && x2_ == x3_ && (x4_ >= 0 || x4_ <= x3_))
     {
-      x1 := x1';
-      x2 := x2';
-      x3 := x3';
-      x4 := x4';
-      x5 := x5';
-      x6 := x6';
-      x7 := x7';
-      x8 := x8';
+      x1 := x1_;
+      x2 := x2_;
+      x3 := x3_;
+      x4 := x4_;
+      x5 := x5_;
+      x6 := x6_;
+      x7 := x7_;
+      x8 := x8_;
     }
   }
   assert(x1 <= 0 && x1 >= x4 + 1 && x2 == x3 && (x4 >= 0 || x4 <= x3));
