dilig-benchmarks/05.desugared.bpl
@@ -1,4 +1,4 @@
-implementation run(flag: bool)
+implementation run(flag: int)
 {
   var x: int;
   var y: int;
@@ -17,6 +17,7 @@ implementation run(flag: bool)
     goto anon4_LoopDone, anon4_LoopBody;
 
   anon4_LoopBody:
+    assume true;
     x := x + 1;
     y := y + 1;
     i := i + x;
@@ -24,15 +25,16 @@ implementation run(flag: bool)
     goto anon5_Then, anon5_Else;
 
   anon5_Else:
-    assume {:partition} !flag;
+    assume {:partition} flag != 0;
     goto anon4_LoopHead;
 
   anon5_Then:
-    assume {:partition} flag;
+    assume {:partition} flag == 0;
     j := j + 1;
     goto anon4_LoopHead;
 
   anon4_LoopDone:
+    assume true;
     assert j >= i;
     return;
 }
