dilig-benchmarks/single/10.desugared.bpl
@@ -17,6 +17,7 @@ implementation main()
     goto anon6_LoopDone, anon6_LoopBody;
 
   anon6_LoopBody:
+    assume true;
     goto anon7_Then, anon7_Else;
 
   anon7_Else:
@@ -43,6 +44,7 @@ implementation main()
     goto anon3;
 
   anon6_LoopDone:
+    assume true;
     assert x == y;
     return;
 }
