dilig-benchmarks/single/13.desugared.bpl
@@ -14,6 +14,7 @@ implementation main()
     goto anon5_LoopDone, anon5_LoopBody;
 
   anon5_LoopBody:
+    assume true;
     goto anon6_Then, anon6_Else;
 
   anon6_Else:
@@ -28,6 +29,7 @@ implementation main()
     goto anon5_LoopHead;
 
   anon5_LoopDone:
+    assume true;
     assert k != 0 ==> j == 2 * k + 2;
     return;
 }
