dilig-benchmarks/single/18.desugared.bpl
@@ -8,39 +8,31 @@ implementation main()
   anon0:
     j := 0;
     b := 0;
-    goto anon6_LoopHead;
+    goto anon5_LoopHead;
 
-  anon6_LoopHead:
-    goto anon6_LoopDone, anon6_LoopBody;
+  anon5_LoopHead:
+    goto anon5_LoopDone, anon5_LoopBody;
 
-  anon6_LoopBody:
+  anon5_LoopBody:
     assume {:partition} b < 100;
-    goto anon7_Then, anon7_Else;
+    goto anon6_Then, anon6_Else;
 
-  anon7_Else:
+  anon6_Else:
     assume {:partition} flag == 0;
     goto anon3;
 
   anon3:
     b := b + 1;
-    goto anon6_LoopHead;
+    goto anon5_LoopHead;
 
-  anon7_Then:
+  anon6_Then:
     assume {:partition} flag != 0;
     j := j + 1;
     goto anon3;
 
-  anon6_LoopDone:
+  anon5_LoopDone:
     assume {:partition} 100 <= b;
-    goto anon8_Then, anon8_Else;
-
-  anon8_Else:
-    assume {:partition} flag == 0;
-    return;
-
-  anon8_Then:
-    assume {:partition} flag != 0;
-    assert j == 100;
+    assert flag != 0 ==> j == 100;
     return;
 }
 
