dilig-benchmarks/single/41.bpl
@@ -6,11 +6,18 @@ procedure main() {
   var n, flag, k, i, j, z : int;
 
   assume(n>=0);
+  /*
   k := 1;
   if(flag != 0) {
     havoc k;
     assume(k>=0);
   }
+  */
+  // Temporarily encoding above if as below assumes
+  // since we don't handle multiple loops yet, and after
+  // desugaring the loops the above if duplicates the loop.
+  assume (flag != 0 ==> k >= 0);
+  assume (flag == 0 ==> k == 1);
   i := 0;
   j := 0;
 
