dilig-benchmarks/single/41.desugared.bpl
@@ -10,37 +10,25 @@ implementation main()
 
   anon0:
     assume n >= 0;
-    k := 1;
-    goto anon5_Then, anon5_Else;
-
-  anon5_Else:
-    assume {:partition} flag == 0;
-    goto anon2;
-
-  anon2:
+    assume flag != 0 ==> k >= 0;
+    assume flag == 0 ==> k == 1;
     i := 0;
     j := 0;
-    goto anon6_LoopHead;
+    goto anon3_LoopHead;
 
-  anon6_LoopHead:
-    goto anon6_LoopDone, anon6_LoopBody;
+  anon3_LoopHead:
+    goto anon3_LoopDone, anon3_LoopBody;
 
-  anon6_LoopBody:
+  anon3_LoopBody:
     assume {:partition} i <= n;
     i := i + 1;
     j := j + i;
-    goto anon6_LoopHead;
+    goto anon3_LoopHead;
 
-  anon6_LoopDone:
+  anon3_LoopDone:
     assume {:partition} n < i;
     z := k + i + j;
     assert z > 2 * n;
     return;
-
-  anon5_Then:
-    assume {:partition} flag != 0;
-    havoc k;
-    assume k >= 0;
-    goto anon2;
 }
 
