dilig-benchmarks/single/42.bpl
@@ -5,11 +5,16 @@ procedure main()
   x  :=  1;
   y  :=  1;
   
+  /*
   if(flag != 0) {
     a  :=  0;
   } else {
     a  :=  1;
   }
+  */
+  // Encoding if as assume to avoid loop duplication in desugaring
+  assume(flag != 0 ==> a == 0);
+  assume(flag == 0 ==> a == 1);
   
   while(*) 
   // invariant (flag == 0 ==> (a mod 2 == 1 && (x+y) mod 2 == 0)) && (flag != 0 ==> (a mod 2 == 0 && (x + y) mod 2 == 0));
@@ -32,10 +37,20 @@ procedure main()
     }
   }
   
-  if(flag != 0) {
-    a := a + 1;
-  }
-
-  assert(a mod 2==1);
+  /*
+   * if(flag != 0) {
+   *   a := a + 1;
+   * }
+   *
+   * assert(a mod 2==1);
+   */
+  /*
+   * Encoding above as simple asserts
+   *  to express postcondition directly after loop.
+   *  This is an engineering limitation of the current
+   *  hacky harness.
+   */
+  assert (flag == 0 ==> (a mod 2 == 1));
+  assert (flag != 0 ==> ((a + 1) mod 2 == 1));
 }
 
