dilig-benchmarks/single/42.desugared.bpl
@@ -9,66 +9,46 @@ implementation main()
   anon0:
     x := 1;
     y := 1;
-    goto anon13_Then, anon13_Else;
+    assume flag != 0 ==> a == 0;
+    assume flag == 0 ==> a == 1;
+    goto anon8_LoopHead;
 
-  anon13_Else:
-    assume {:partition} flag == 0;
-    a := 1;
-    goto anon3;
+  anon8_LoopHead:
+    goto anon8_LoopDone, anon8_LoopBody;
 
-  anon3:
-    goto anon14_LoopHead;
+  anon8_LoopBody:
+    assume true;
+    goto anon9_Then, anon9_Else;
 
-  anon14_LoopHead:
-    goto anon14_LoopDone, anon14_LoopBody;
-
-  anon14_LoopBody:
-    goto anon15_Then, anon15_Else;
-
-  anon15_Else:
+  anon9_Else:
     assume {:partition} flag == 0;
     a := x + y + 1;
     y := y + 1;
-    goto anon7;
+    goto anon4;
 
-  anon7:
-    goto anon16_Then, anon16_Else;
+  anon4:
+    goto anon10_Then, anon10_Else;
 
-  anon16_Else:
+  anon10_Else:
     assume {:partition} a mod 2 != 1;
     x := x + 1;
-    goto anon14_LoopHead;
+    goto anon8_LoopHead;
 
-  anon16_Then:
+  anon10_Then:
     assume {:partition} a mod 2 == 1;
     y := y + 1;
-    goto anon14_LoopHead;
+    goto anon8_LoopHead;
 
-  anon15_Then:
+  anon9_Then:
     assume {:partition} flag != 0;
     a := x + y;
     x := x + 1;
-    goto anon7;
+    goto anon4;
 
-  anon14_LoopDone:
-    goto anon17_Then, anon17_Else;
-
-  anon17_Else:
-    assume {:partition} flag == 0;
-    goto anon12;
-
-  anon12:
-    assert a mod 2 == 1;
+  anon8_LoopDone:
+    assume true;
+    assert flag == 0 ==> a mod 2 == 1;
+    assert flag != 0 ==> (a + 1) mod 2 == 1;
     return;
-
-  anon17_Then:
-    assume {:partition} flag != 0;
-    a := a + 1;
-    goto anon12;
-
-  anon13_Then:
-    assume {:partition} flag != 0;
-    a := 0;
-    goto anon3;
 }
 
