dilig-benchmarks/single/44.desugared.bpl
@@ -10,34 +10,23 @@ implementation main()
   anon0:
     i := 0;
     j := 0;
-    goto anon6_Then, anon6_Else;
-
-  anon6_Else:
-    assume {:partition} flag != 1;
-    n := 2;
-    goto anon3;
-
-  anon3:
+    assume flag == 1 ==> n == 1;
+    assume flag != 1 ==> n == 2;
     i := 0;
-    goto anon7_LoopHead;
+    goto anon3_LoopHead;
 
-  anon7_LoopHead:
-    goto anon7_LoopDone, anon7_LoopBody;
+  anon3_LoopHead:
+    goto anon3_LoopDone, anon3_LoopBody;
 
-  anon7_LoopBody:
+  anon3_LoopBody:
     assume {:partition} i <= k;
     i := i + 1;
     j := j + n;
-    goto anon7_LoopHead;
+    goto anon3_LoopHead;
 
-  anon7_LoopDone:
+  anon3_LoopDone:
     assume {:partition} k < i;
     assert flag == 1 ==> j == i;
     return;
-
-  anon6_Then:
-    assume {:partition} flag == 1;
-    n := 1;
-    goto anon3;
 }
 
