ice-benchmarks/single/fig3.dimo.bpl
@@ -1,16 +1,21 @@
 // ../ice-benchmarks/single/fig3.c
 procedure main()
 {
-  var x, y, lock: int;
+  var x, y, lock, choice: int;
   lock := 0;
 
   lock := 1;
+  /*
   x := y;
   if (*)
   {
     lock := 0;
     y := y + 1;
   }
+  */
+  // Encoding above if as assumes to avoid loop duplication in desugaring
+  assume (choice == 0 ==> (lock == 0 && y == x + 1));
+  assume (choice != 0 ==> (lock == 1 && y == x));
 
   while (x != y)
   // invariant (x == y ==> lock == 1);
