ice-benchmarks/single/inc.desugared.dimo.bpl
@@ -1,1 +1,25 @@
-x <= 100
+implementation main()
+{
+  var x: int;
+  var m: int;
+
+
+  anon0:
+    x := 0;
+    goto anon3_LoopHead;
+
+  anon3_LoopHead:
+    goto anon3_LoopDone, anon3_LoopBody;
+
+  anon3_LoopBody:
+    assume {:partition} x < 100;
+    havoc m;
+    x := x + 1;
+    goto anon3_LoopHead;
+
+  anon3_LoopDone:
+    assume {:partition} 100 <= x;
+    assert x == 100;
+    return;
+}
+
