ice-benchmarks/single/inc2.desugared.dimo.bpl
@@ -1,1 +1,24 @@
-(N >= 0) ==> x <= N
+implementation main()
+{
+  var x: int;
+  var N: int;
+
+
+  anon0:
+    x := 0;
+    goto anon3_LoopHead;
+
+  anon3_LoopHead:
+    goto anon3_LoopDone, anon3_LoopBody;
+
+  anon3_LoopBody:
+    assume {:partition} x < N;
+    x := x + 1;
+    goto anon3_LoopHead;
+
+  anon3_LoopDone:
+    assume {:partition} N <= x;
+    assert N < 0 || x == N;
+    return;
+}
+
