ice-benchmarks/single/tacas6.desugared.dimo.bpl
@@ -1,1 +1,28 @@
-i - j == x - y
+implementation main()
+{
+  var x: int;
+  var y: int;
+  var i: int;
+  var j: int;
+
+
+  anon0:
+    x := i;
+    y := j;
+    goto anon3_LoopHead;
+
+  anon3_LoopHead:
+    goto anon3_LoopDone, anon3_LoopBody;
+
+  anon3_LoopBody:
+    assume {:partition} x != 0;
+    x := x - 1;
+    y := y - 1;
+    goto anon3_LoopHead;
+
+  anon3_LoopDone:
+    assume {:partition} x == 0;
+    assert i == j ==> y == 0;
+    return;
+}
+
